src/KZG_BatchOpening_knowledge_soundness.thy
@@ -30,7 +30,7 @@ type_synonym ('a', 'e') extractor =
 definition knowledge_soundness_game :: "('a, 'e) extractor \<Rightarrow> ('a, 'e) adversary_1 \<Rightarrow> ('a, 'e) adversary_2 
   \<Rightarrow> bool spmf"
   where "knowledge_soundness_game E \<A> \<A>' = TRY do {
-  PK \<leftarrow> key_gen;
+  PK \<leftarrow> KeyGen;
   (C,calc_vec) \<leftarrow> \<A> PK;
   _ :: unit \<leftarrow> assert_spmf (length PK = length calc_vec 
                           \<and> C = fold (\<lambda> i acc. acc \<otimes>\<^bsub>G\<^sub>p\<^esub> PK!i ^\<^bsub>G\<^sub>p\<^esub> (calc_vec!i)) [0..<length PK] \<one>\<^bsub>G\<^sub>p\<^esub>);  
@@ -124,12 +124,12 @@ proof -
   then show ?thesis by presburger
 qed
 
-lemma key_gen_alt_def: "key_gen = do {
+lemma key_gen_alt_def: "KeyGen = do {
     x :: nat \<leftarrow> sample_uniform (order G\<^sub>p);
     let \<alpha>::'e mod_ring = of_int_mod_ring (int x) in
     return_spmf (map (\<lambda>t. \<^bold>g\<^bsub>G\<^sub>p\<^esub> ^\<^bsub>G\<^sub>p\<^esub> (\<alpha>^t)) [0..<max_deg+1])
   }"
-  unfolding key_gen_def Setup_def Let_def split_def by simp
+  unfolding KeyGen_def Setup_def Let_def split_def by simp
 
 lemma knowledge_soundness_game_alt_def: 
   "knowledge_soundness_game E \<A> \<A>' = 
@@ -151,7 +151,7 @@ lemma knowledge_soundness_game_alt_def:
 proof -
   note [simp] = Let_def split_def
   have "do {
-  PK \<leftarrow> key_gen;
+  PK \<leftarrow> KeyGen;
   (C,calc_vec) \<leftarrow> \<A> PK;
   _ :: unit \<leftarrow> assert_spmf (length PK = length calc_vec 
                           \<and> C = fold (\<lambda> i acc. acc \<otimes>\<^bsub>G\<^sub>p\<^esub> PK!i ^\<^bsub>G\<^sub>p\<^esub> (calc_vec!i)) [0..<length PK] \<one>\<^bsub>G\<^sub>p\<^esub>);  
@@ -160,17 +160,17 @@ proof -
   return_spmf (VerifyEvalBatch PK C B r_x w_B \<and> poly r_x i \<noteq> poly (E C calc_vec) i)} 
   = 
   do {
-  PK \<leftarrow> key_gen;
+  PK \<leftarrow> KeyGen;
   (C,calc_vec) \<leftarrow> \<A> PK;
   (i, B, r_x, w_B) \<leftarrow> \<A>' PK C calc_vec;
   _ :: unit \<leftarrow> assert_spmf (length PK = length calc_vec 
                           \<and> C = fold (\<lambda> i acc. acc \<otimes>\<^bsub>G\<^sub>p\<^esub> PK!i ^\<^bsub>G\<^sub>p\<^esub> (calc_vec!i)) [0..<length PK] \<one>\<^bsub>G\<^sub>p\<^esub>);  
   _ :: unit \<leftarrow> assert_spmf (i \<in> B  \<and> valid_batch_msg r_x w_B B);  
   return_spmf (VerifyEvalBatch PK C B r_x w_B \<and> poly r_x i \<noteq> poly (E C calc_vec) i)}"
-    using pull_down_assert_spmf_with_return[of key_gen \<A>] by fastforce
+    using pull_down_assert_spmf_with_return[of KeyGen \<A>] by fastforce
   then have "knowledge_soundness_game E \<A> \<A>' = 
   TRY do {
-    PK \<leftarrow> key_gen;
+    PK \<leftarrow> KeyGen;
     (C,calc_vec) \<leftarrow> \<A> PK;
     let \<phi> = E C calc_vec;
     (i, B, r_x, w_B) \<leftarrow> \<A>' PK C calc_vec;
@@ -181,7 +181,7 @@ proof -
   } ELSE return_spmf False"
     unfolding knowledge_soundness_game_def by algebra
   also have "\<dots> = TRY do {
-    PK \<leftarrow> key_gen;
+    PK \<leftarrow> KeyGen;
     TRY do {
     (C,calc_vec) \<leftarrow> \<A> PK;
     TRY do {
@@ -203,7 +203,7 @@ proof -
    unfolding split_def Let_def
    by (fold try_bind_spmf_lossless2[OF lossless_return_spmf])simp
   also have "\<dots> = TRY do {
-    PK \<leftarrow> key_gen;
+    PK \<leftarrow> KeyGen;
     TRY do {
     (C,calc_vec) \<leftarrow> \<A> PK;
     TRY do {
@@ -225,7 +225,7 @@ proof -
   } ELSE return_spmf False"
    by(auto simp add: try_bind_assert_spmf try_spmf_return_spmf1 intro!: try_spmf_cong bind_spmf_cong)
   also have "\<dots> = TRY do {
-    PK \<leftarrow> key_gen;
+    PK \<leftarrow> KeyGen;
     TRY do {
     (C,calc_vec) \<leftarrow> \<A> PK;
     TRY do {
@@ -247,7 +247,7 @@ proof -
   } ELSE return_spmf False"
     using assert_anding by presburger
    also have "\<dots> = TRY do {
-    PK \<leftarrow> key_gen;
+    PK \<leftarrow> KeyGen;
     TRY do {
     (C,calc_vec) \<leftarrow> \<A> PK;
     TRY do {
@@ -268,7 +268,7 @@ proof -
     unfolding split_def Let_def
     by(fold try_bind_spmf_lossless2[OF lossless_return_spmf]) simp
    also have "\<dots> = TRY do {
-    PK \<leftarrow> key_gen;
+    PK \<leftarrow> KeyGen;
     TRY do {
     (C,calc_vec) \<leftarrow> \<A> PK;
     TRY do {
@@ -289,7 +289,7 @@ proof -
      using assert_anding by presburger
    text \<open>next step, add assert PK construction\<close>
   also have "\<dots> = TRY do {
-    PK \<leftarrow> key_gen;
+    PK \<leftarrow> KeyGen;
     (C,calc_vec) \<leftarrow> \<A> PK;
     let \<phi> = E C calc_vec;
     (i, B, r_x, w_B) \<leftarrow> \<A>' PK C calc_vec;
@@ -354,7 +354,7 @@ lemma bind_game_knowledge_soundness_reduction_alt_def:
     } ELSE return_spmf False"
 proof -
   have "bind_game (knowledge_soundness_reduction E \<A> \<A>') = TRY do {
-  PK \<leftarrow> key_gen;
+  PK \<leftarrow> KeyGen;
   (C, i, \<phi>_i, w_i, B, w_B, r_x) \<leftarrow> (knowledge_soundness_reduction E \<A> \<A>') PK;
   _ :: unit \<leftarrow> assert_spmf (i \<in> B \<and> \<phi>_i \<noteq> poly r_x i \<and> valid_msg \<phi>_i w_i \<and> valid_batch_msg r_x w_B B); 
   let b = VerifyEval PK C i \<phi>_i w_i;
@@ -363,7 +363,7 @@ proof -
   return_spmf True} ELSE return_spmf False" 
     by (fact bind_game_alt_def)
   also have "\<dots> = TRY do {
-  PK \<leftarrow> key_gen;
+  PK \<leftarrow> KeyGen;
   (C,calc_vec) \<leftarrow> \<A> PK;
   _ :: unit \<leftarrow> assert_spmf (length PK = length calc_vec 
                           \<and> C = fold (\<lambda> i acc. acc \<otimes>\<^bsub>G\<^sub>p\<^esub> PK!i ^\<^bsub>G\<^sub>p\<^esub> (calc_vec!i)) [0..<length PK] \<one>\<^bsub>G\<^sub>p\<^esub>);  
@@ -378,7 +378,7 @@ proof -
   return_spmf True} ELSE return_spmf False"
   unfolding knowledge_soundness_reduction_def by (simp add: split_def Let_def)
   also have "\<dots> = TRY do {
-    PK \<leftarrow> key_gen;
+    PK \<leftarrow> KeyGen;
     TRY do{
     (C,calc_vec) \<leftarrow> \<A> PK;
     TRY do {
@@ -403,7 +403,7 @@ proof -
    unfolding split_def Let_def 
    by(fold try_bind_spmf_lossless2[OF lossless_return_spmf]) simp
   also have "\<dots> = TRY do {
-    PK \<leftarrow> key_gen;
+    PK \<leftarrow> KeyGen;
     TRY do{
     (C,calc_vec) \<leftarrow> \<A> PK;
     TRY do {
@@ -426,7 +426,7 @@ proof -
   } ELSE return_spmf False"
     using assert_anding by presburger
   also have "\<dots> = TRY do {
-    PK \<leftarrow> key_gen;
+    PK \<leftarrow> KeyGen;
     (C,calc_vec) \<leftarrow> \<A> PK;
     _ :: unit \<leftarrow> assert_spmf (length PK = length calc_vec 
                             \<and> C = fold (\<lambda> i acc. acc \<otimes>\<^bsub>G\<^sub>p\<^esub> PK!i ^\<^bsub>G\<^sub>p\<^esub> (calc_vec!i)) [0..<length PK] \<one>\<^bsub>G\<^sub>p\<^esub>);  
@@ -442,7 +442,7 @@ proof -
    unfolding split_def Let_def 
    by(fold try_bind_spmf_lossless2[OF lossless_return_spmf]) simp
   also have "\<dots> = TRY do {
-    PK \<leftarrow> key_gen;
+    PK \<leftarrow> KeyGen;
     (C,calc_vec) \<leftarrow> \<A> PK;
     
     (i, B, r_x, w_B) \<leftarrow> \<A>' PK C calc_vec;
@@ -458,7 +458,7 @@ proof -
   } ELSE return_spmf False"
   proof -
     have "do {
-    PK \<leftarrow> key_gen;
+    PK \<leftarrow> KeyGen;
     (C,calc_vec) \<leftarrow> \<A> PK;
     _ :: unit \<leftarrow> assert_spmf (length PK = length calc_vec 
                             \<and> C = fold (\<lambda> i acc. acc \<otimes>\<^bsub>G\<^sub>p\<^esub> PK!i ^\<^bsub>G\<^sub>p\<^esub> (calc_vec!i)) [0..<length PK] \<one>\<^bsub>G\<^sub>p\<^esub>);  
@@ -471,7 +471,7 @@ proof -
                             \<and> VerifyEval PK C i \<phi>_i w_i \<and> VerifyEvalBatch PK C B r_x w_B);
     return_spmf True
     } = do {
-    PK \<leftarrow> key_gen;
+    PK \<leftarrow> KeyGen;
     (C,calc_vec) \<leftarrow> \<A> PK;
     
     (i, B, r_x, w_B) \<leftarrow> \<A>' PK C calc_vec;
@@ -485,12 +485,12 @@ proof -
                             \<and> VerifyEval PK C i \<phi>_i w_i \<and> VerifyEvalBatch PK C B r_x w_B);
     return_spmf True
     }"
-      using pull_down_assert_spmf_with_assert[of key_gen \<A>] 
+      using pull_down_assert_spmf_with_assert[of KeyGen \<A>] 
       by (simp add: Let_def split_def)
     then show ?thesis by argo
   qed
   also have "\<dots> = TRY do {
-    PK \<leftarrow> key_gen;
+    PK \<leftarrow> KeyGen;
     TRY do {
     (C,calc_vec) \<leftarrow> \<A> PK;
     TRY do {
@@ -512,7 +512,7 @@ proof -
   unfolding split_def Let_def 
   by(fold try_bind_spmf_lossless2[OF lossless_return_spmf]) simp
   also have "\<dots> = TRY do {
-    PK \<leftarrow> key_gen;
+    PK \<leftarrow> KeyGen;
     TRY do {
     (C,calc_vec) \<leftarrow> \<A> PK;
     TRY do {
@@ -534,7 +534,7 @@ proof -
     unfolding Let_def
     using assert_anding by presburger
   also have "\<dots> = TRY do {
-    PK \<leftarrow> key_gen;
+    PK \<leftarrow> KeyGen;
     (C,calc_vec) \<leftarrow> \<A> PK;
     (i, B, r_x, w_B) \<leftarrow> \<A>' PK C calc_vec;
     let \<phi> = E C calc_vec;
