src/KZG_knowledge_soundness.thy
@@ -32,7 +32,7 @@ type_synonym ('a', 'e') extractor =
 definition knowledge_soundness_game :: "('a, 'e) extractor \<Rightarrow> ('a, 'e) adversary_1 \<Rightarrow> ('a, 'e) adversary_2 
   \<Rightarrow> bool spmf"
   where "knowledge_soundness_game E \<A> \<A>' = TRY do {
-  PK \<leftarrow> key_gen;
+  PK \<leftarrow> KeyGen;
   (C,calc_vec) \<leftarrow> \<A> PK;
   _ :: unit \<leftarrow> assert_spmf (length PK = length calc_vec 
                           \<and> C = fold (\<lambda> i acc. acc \<otimes>\<^bsub>G\<^sub>p\<^esub> PK!i ^\<^bsub>G\<^sub>p\<^esub> (calc_vec!i)) [0..<length PK] \<one>\<^bsub>G\<^sub>p\<^esub>);  
@@ -127,12 +127,12 @@ proof -
   then show ?thesis by presburger
 qed
 
-lemma key_gen_alt_def: "key_gen = do {
+lemma key_gen_alt_def: "KeyGen = do {
     x :: nat \<leftarrow> sample_uniform (order G\<^sub>p);
     let \<alpha>::'e mod_ring = of_int_mod_ring (int x) in
     return_spmf (map (\<lambda>t. \<^bold>g\<^bsub>G\<^sub>p\<^esub> ^\<^bsub>G\<^sub>p\<^esub> (\<alpha>^t)) [0..<max_deg+1])
   }"
-  unfolding key_gen_def Setup_def Let_def split_def by simp
+  unfolding KeyGen_def Setup_def Let_def split_def by simp
 
 lemma knowledge_soundness_game_alt_def: 
   "knowledge_soundness_game E \<A> \<A>' = 
@@ -152,7 +152,7 @@ lemma knowledge_soundness_game_alt_def:
 proof -
   note [simp] = Let_def split_def
   have "do {
-  PK \<leftarrow> key_gen;
+  PK \<leftarrow> KeyGen;
   (C,calc_vec) \<leftarrow> \<A> PK;
   _ :: unit \<leftarrow> assert_spmf (length PK = length calc_vec 
                           \<and> C = fold (\<lambda> i acc. acc \<otimes>\<^bsub>G\<^sub>p\<^esub> PK!i ^\<^bsub>G\<^sub>p\<^esub> (calc_vec!i)) [0..<length PK] \<one>\<^bsub>G\<^sub>p\<^esub>);  
@@ -161,17 +161,17 @@ proof -
   return_spmf (VerifyEval PK C i \<phi>_i w_i \<and> \<phi>_i \<noteq> poly (E C calc_vec) i)} 
   = 
   do {
-  PK \<leftarrow> key_gen;
+  PK \<leftarrow> KeyGen;
   (C,calc_vec) \<leftarrow> \<A> PK;
   (i, \<phi>_i, w_i) \<leftarrow> \<A>' PK C calc_vec;
   _ :: unit \<leftarrow> assert_spmf (length PK = length calc_vec 
                           \<and> C = fold (\<lambda> i acc. acc \<otimes>\<^bsub>G\<^sub>p\<^esub> PK!i ^\<^bsub>G\<^sub>p\<^esub> (calc_vec!i)) [0..<length PK] \<one>\<^bsub>G\<^sub>p\<^esub>);  
   _ :: unit \<leftarrow> assert_spmf (valid_msg \<phi>_i w_i);  
   return_spmf (VerifyEval PK C i \<phi>_i w_i \<and> \<phi>_i \<noteq> poly (E C calc_vec) i)}"
-    using pull_down_assert_spmf_with_return[of key_gen \<A>] by fastforce
+    using pull_down_assert_spmf_with_return[of KeyGen \<A>] by fastforce
   then have "knowledge_soundness_game E \<A> \<A>' = 
   TRY do {
-    PK \<leftarrow> key_gen;
+    PK \<leftarrow> KeyGen;
     (C,calc_vec) \<leftarrow> \<A> PK;
     let \<phi> = E C calc_vec;
     (i, \<phi>_i, w_i) \<leftarrow> \<A>' PK C calc_vec;
@@ -182,7 +182,7 @@ proof -
   } ELSE return_spmf False"
     unfolding knowledge_soundness_game_def by algebra
   also have "\<dots> = TRY do {
-    PK \<leftarrow> key_gen;
+    PK \<leftarrow> KeyGen;
     TRY do {
     (C,calc_vec) \<leftarrow> \<A> PK;
     TRY do {
@@ -204,7 +204,7 @@ proof -
    unfolding split_def Let_def
    by (fold try_bind_spmf_lossless2[OF lossless_return_spmf])simp
   also have "\<dots> = TRY do {
-    PK \<leftarrow> key_gen;
+    PK \<leftarrow> KeyGen;
     TRY do {
     (C,calc_vec) \<leftarrow> \<A> PK;
     TRY do {
@@ -226,7 +226,7 @@ proof -
   } ELSE return_spmf False"
    by(auto simp add: try_bind_assert_spmf try_spmf_return_spmf1 intro!: try_spmf_cong bind_spmf_cong)
   also have "\<dots> = TRY do {
-    PK \<leftarrow> key_gen;
+    PK \<leftarrow> KeyGen;
     TRY do {
     (C,calc_vec) \<leftarrow> \<A> PK;
     TRY do {
@@ -248,7 +248,7 @@ proof -
   } ELSE return_spmf False"
     using assert_anding by presburger
    also have "\<dots> = TRY do {
-    PK \<leftarrow> key_gen;
+    PK \<leftarrow> KeyGen;
     TRY do {
     (C,calc_vec) \<leftarrow> \<A> PK;
     TRY do {
@@ -269,7 +269,7 @@ proof -
     unfolding split_def Let_def
     by(fold try_bind_spmf_lossless2[OF lossless_return_spmf]) simp
    also have "\<dots> = TRY do {
-    PK \<leftarrow> key_gen;
+    PK \<leftarrow> KeyGen;
     TRY do {
     (C,calc_vec) \<leftarrow> \<A> PK;
     TRY do {
@@ -373,7 +373,7 @@ lemma bind_game_knowledge_soundness_reduction_alt_def:
     } ELSE return_spmf False"
 proof -
   have "bind_game (knowledge_soundness_reduction E \<A> \<A>') = TRY do {
-  PK \<leftarrow> key_gen;
+  PK \<leftarrow> KeyGen;
   (C, i, \<phi>_i, w_i, \<phi>'_i, w'_i) \<leftarrow> (knowledge_soundness_reduction E \<A> \<A>') PK;
   _ :: unit \<leftarrow> assert_spmf (\<phi>_i \<noteq> \<phi>'_i \<and> valid_msg \<phi>_i w_i \<and> valid_msg \<phi>'_i w'_i);
   let b = VerifyEval PK C i \<phi>_i w_i;
@@ -382,7 +382,7 @@ proof -
   return_spmf True } ELSE return_spmf False" 
     by (fact bind_game_alt_def)
   also have "\<dots> = TRY do {
-  PK \<leftarrow> key_gen;
+  PK \<leftarrow> KeyGen;
   (C,calc_vec) \<leftarrow> \<A> PK;
   _ :: unit \<leftarrow> assert_spmf (length PK = length calc_vec 
                           \<and> C = fold (\<lambda> i acc. acc \<otimes>\<^bsub>G\<^sub>p\<^esub> PK!i ^\<^bsub>G\<^sub>p\<^esub> (calc_vec!i)) [0..<length PK] \<one>\<^bsub>G\<^sub>p\<^esub>);  
@@ -398,7 +398,7 @@ proof -
   return_spmf True } ELSE return_spmf False"
   unfolding knowledge_soundness_reduction_def by (simp add: split_def Let_def)
   also have "\<dots> =  TRY do {
-    PK \<leftarrow> key_gen;
+    PK \<leftarrow> KeyGen;
     TRY do {
     (C,calc_vec) \<leftarrow> \<A> PK;
     TRY do {
@@ -426,7 +426,7 @@ proof -
    unfolding split_def Let_def 
    by(fold try_bind_spmf_lossless2[OF lossless_return_spmf]) simp
   also have "\<dots> = TRY do {
-    PK \<leftarrow> key_gen;
+    PK \<leftarrow> KeyGen;
     TRY do {
     (C,calc_vec) \<leftarrow> \<A> PK;
     TRY do {
@@ -454,7 +454,7 @@ proof -
     } ELSE return_spmf False"
     using assert_anding by presburger
   also have "\<dots> = TRY do {
-    PK \<leftarrow> key_gen;
+    PK \<leftarrow> KeyGen;
     TRY do {
     (C,calc_vec) \<leftarrow> \<A> PK;
     TRY do {
@@ -481,7 +481,7 @@ proof -
    unfolding split_def Let_def 
    by(fold try_bind_spmf_lossless2[OF lossless_return_spmf]) simp
   also have "\<dots> = TRY do {
-    PK \<leftarrow> key_gen;
+    PK \<leftarrow> KeyGen;
     TRY do {
     (C,calc_vec) \<leftarrow> \<A> PK;
     TRY do {
@@ -521,7 +521,7 @@ proof -
     then show ?thesis using assert_anding by algebra
   qed
   also have "\<dots> =  TRY do {
-    PK \<leftarrow> key_gen;
+    PK \<leftarrow> KeyGen;
     (C,calc_vec) \<leftarrow> \<A> PK;
     _ :: unit \<leftarrow> assert_spmf (length PK = length calc_vec 
             \<and> C = fold (\<lambda> i acc. acc \<otimes>\<^bsub>G\<^sub>p\<^esub> PK!i ^\<^bsub>G\<^sub>p\<^esub> (calc_vec!i)) [0..<length PK] \<one>\<^bsub>G\<^sub>p\<^esub>);  
@@ -536,7 +536,7 @@ proof -
     unfolding split_def Let_def 
     by(fold try_bind_spmf_lossless2[OF lossless_return_spmf]) simp
   also have "\<dots> =  TRY do {
-    PK \<leftarrow> key_gen;
+    PK \<leftarrow> KeyGen;
     (C,calc_vec) \<leftarrow> \<A> PK;
     (i, \<phi>_i, w_i) \<leftarrow> \<A>' PK C calc_vec;
     _ :: unit \<leftarrow> assert_spmf (length PK = length calc_vec 
@@ -550,7 +550,7 @@ proof -
     } ELSE return_spmf False"
   proof -
     have "do {
-    PK \<leftarrow> key_gen;
+    PK \<leftarrow> KeyGen;
     (C,calc_vec) \<leftarrow> \<A> PK;
     _ :: unit \<leftarrow> assert_spmf (length PK = length calc_vec 
             \<and> C = fold (\<lambda> i acc. acc \<otimes>\<^bsub>G\<^sub>p\<^esub> PK!i ^\<^bsub>G\<^sub>p\<^esub> (calc_vec!i)) [0..<length PK] \<one>\<^bsub>G\<^sub>p\<^esub>);  
@@ -562,7 +562,7 @@ proof -
                             \<and> VerifyEval PK C i (poly (E C calc_vec) i) (createWitness PK (E C calc_vec) i));
     return_spmf True
     } = do {
-    PK \<leftarrow> key_gen;
+    PK \<leftarrow> KeyGen;
     (C,calc_vec) \<leftarrow> \<A> PK;
     (i, \<phi>_i, w_i) \<leftarrow> \<A>' PK C calc_vec;
     _ :: unit \<leftarrow> assert_spmf (length PK = length calc_vec 
@@ -574,12 +574,12 @@ proof -
                             \<and> VerifyEval PK C i (poly (E C calc_vec) i) (createWitness PK (E C calc_vec) i));
     return_spmf True
     }"
-      using pull_down_assert_spmf_with_assert[of key_gen \<A>] 
+      using pull_down_assert_spmf_with_assert[of KeyGen \<A>] 
       by (simp add: Let_def split_def)
     then show ?thesis by argo
   qed
   also have "\<dots> =  TRY do {
-    PK \<leftarrow> key_gen;
+    PK \<leftarrow> KeyGen;
     TRY do {
     (C,calc_vec) \<leftarrow> \<A> PK;
     TRY do {
@@ -600,7 +600,7 @@ proof -
   unfolding split_def Let_def 
   by(fold try_bind_spmf_lossless2[OF lossless_return_spmf]) simp
   also have "\<dots> = TRY do {
-    PK \<leftarrow> key_gen;
+    PK \<leftarrow> KeyGen;
     TRY do {
     (C,calc_vec) \<leftarrow> \<A> PK;
     TRY do {
@@ -620,7 +620,7 @@ proof -
     } ELSE return_spmf False"
     using assert_anding by presburger
   also have "\<dots> = TRY do {
-    PK \<leftarrow> key_gen;
+    PK \<leftarrow> KeyGen;
     (C,calc_vec) \<leftarrow> \<A> PK;
     let \<phi> = E C calc_vec;
     (i, \<phi>_i, w_i) \<leftarrow> \<A>' PK C calc_vec;
